examples/layeredeffects/ID3.fst
@@ -6,13 +6,13 @@ let w0 a = (a -> Type0) -> Type0
 
 // We require monotonicity of them
 let monotonic (w:w0 'a) =
-  forall p1 p2. (forall x. p1 x ==> p2 x) ==> w p1 ==> w p2
+  forall p1 p2. {:nopattern (* override *)} (forall x. {:nopattern (* override *)} p1 x ==> p2 x) ==> w p1 ==> w p2
 
 val w (a : Type u#a) : Type u#(max 1 a)
 let w a = pure_wp a
 
 let repr (a : Type) (wp : w a) : Type =
-  v:a{forall p. wp p ==> p v}
+  v:a{forall p. {:nopattern (* override *)} wp p ==> p v}
 
 open FStar.Monotonic.Pure
 
@@ -21,8 +21,9 @@ let return (a : Type) (x : a) : repr a (as_pure_wp (fun p -> p x)) =
 
 unfold
 let bind_wp (#a:Type u#a) (#b:Type u#b) (wp_v:w a) (wp_f:a -> w b) : w b =
-  elim_pure_wp_monotonicity_forall u#a ();
-  elim_pure_wp_monotonicity_forall u#b ();
+  elim_pure_wp_monotonicity wp_v;
+  introduce forall (x:a). is_monotonic (wp_f x)
+  with elim_pure_wp_monotonicity (wp_f x);
   as_pure_wp (fun p -> wp_v (fun x -> wp_f x p))
 
 let bind (a b : Type) (wp_v : w a) (wp_f: a -> w b)
@@ -34,13 +35,14 @@ let bind (a b : Type) (wp_v : w a) (wp_f: a -> w b)
 let subcomp (a:Type) (wp1 wp2: w a)
     (f : repr a wp1)
 : Pure (repr a wp2)
-       (requires (forall p. wp2 p ==> wp1 p))
+       (requires (forall p. {:nopattern (* override *)} wp2 p ==> wp1 p))
        (ensures fun _ -> True)
 = f
 
 unfold
 let if_then_else_wp (#a:Type u#a) (wp1 wp2:w a) (p:bool) =
-  elim_pure_wp_monotonicity_forall u#a ();
+  elim_pure_wp_monotonicity wp1;
+  elim_pure_wp_monotonicity wp2;
   as_pure_wp (fun post -> (p ==> wp1 post) /\ ((~p) ==> wp2 post))
 
 let if_then_else (a : Type) (wp1 wp2 : w a) (f : repr a wp1) (g : repr a wp2) (p : bool) : Type =
@@ -77,7 +79,7 @@ let l () : int =
   reify (test_f ())
 
 effect Id (a:Type) (pre:pure_pre) (post:pure_post' a pre) =
-        ID a (as_pure_wp (fun (p:pure_post a) -> pre /\ (forall (pure_result:a). post pure_result ==> p pure_result)))
+        ID a (as_pure_wp (fun (p:pure_post a) -> pre /\ (forall (pure_result:a). {:nopattern (* override *)} post pure_result ==> p pure_result)))
 
 effect IdT (a:Type) = Id a True (fun _ -> True)
 
