examples/layeredeffects/ND.fst
@@ -37,9 +37,10 @@ let w_return x = as_pure_wp (fun p -> p x)
 unfold
 val w_bind (#a:Type u#a) (#b : Type u#b) : w a -> (a -> w b) -> w b
 unfold
-let w_bind wp1 k =
-  elim_pure_wp_monotonicity_forall u#a ();
-  elim_pure_wp_monotonicity_forall u#b ();
+let w_bind (#a:Type u#a) (#b : Type u#b) wp1 k =
+  elim_pure_wp_monotonicity wp1;
+  introduce forall (x:a). is_monotonic (k x)
+  with elim_pure_wp_monotonicity (k x);
   as_pure_wp (fun p -> wp1 (fun x -> k x p))
 
 val interp (#a : Type) : m a -> w a
@@ -118,7 +119,8 @@ let ibind (a : Type) (b : Type) (wp_v : w a) (wp_f: a -> w b) (v : irepr a wp_v)
 let isubcomp (a:Type) (wp1 wp2: w a) (f : irepr a wp1) : Pure (irepr a wp2) (requires w_ord wp2 wp1) (ensures fun _ -> True) = f
 
 let wp_if_then_else (#a:Type u#a) (wp1 wp2:w a) (b:bool) : w a=
-  elim_pure_wp_monotonicity_forall u#a ();
+  elim_pure_wp_monotonicity wp1;
+  elim_pure_wp_monotonicity wp2;
   as_pure_wp (fun p -> (b ==> wp1 p) /\ ((~b) ==> wp2 p))
 
 let i_if_then_else (a : Type) (wp1 wp2 : w a) (f : irepr a wp1) (g : irepr a wp2) (b : bool) : Type =
