tests/bug-reports/closed/Bug2169.fst
@@ -24,13 +24,13 @@ val w0 (a : Type u#a) : Type u#(max 1 a)
 let w0 a = (a -> Type0) -> Type0
 
 let monotonic (w:w0 'a) =
-  forall p1 p2. (forall x. p1 x ==> p2 x) ==> w p1 ==> w p2
+  forall p1 p2. {:nopattern (* override *)} (forall x. {:nopattern (* override *)} p1 x ==> p2 x) ==> w p1 ==> w p2
 
 val w (a : Type u#a) : Type u#(max 1 a)
 let w a = pure_wp a
 
 val w_ord (#a : Type) : w a -> w a -> Type0
-let w_ord wp1 wp2 = forall p. wp1 p ==> wp2 p
+let w_ord wp1 wp2 = forall p. {:nopattern (* override *)} wp1 p ==> wp2 p
 
 unfold
 val w_return (#a : Type) : a -> w a
@@ -41,12 +41,13 @@ unfold
 val w_bind (#a #b : Type) : w a -> (a -> w b) -> w b
 unfold
 let w_bind (#a:Type u#a) (#b : Type u#b) wp1 k =
-  elim_pure_wp_monotonicity_forall u#a ();
-  elim_pure_wp_monotonicity_forall u#b ();
+  elim_pure_wp_monotonicity wp1;
+  introduce forall (x:a). is_monotonic (k x)
+  with elim_pure_wp_monotonicity (k x);
   as_pure_wp (fun p -> wp1 (fun x -> k x p))
 
 val interp (#a : Type) : m a -> w a
-let interp #a (l:list a) = as_pure_wp (fun p -> forall x. memP x l ==> p x)
+let interp #a (l:list a) = as_pure_wp (fun p -> forall x. {:nopattern (* override *)} memP x l ==> p x)
 
 val concatlemma (#a:Type) (l1 l2 :list a) (x:a) : Lemma (memP x (l1@l2) <==> memP x l1 \/ memP x l2)
 let rec concatlemma #a l1 l2 x =
@@ -55,7 +56,7 @@ let rec concatlemma #a l1 l2 x =
   | h::t -> concatlemma t l2 x
 
 val concatmaplemma : (#a:Type) -> (#b:Type) -> l:list a -> (f:(a -> list b)) -> x:b ->
-                               Lemma (memP x (concatMap f l) <==> (exists a. memP a l /\ memP x (f a)))
+                               Lemma (memP x (concatMap f l) <==> (exists a. {:nopattern (* override *)} memP a l /\ memP x (f a)))
                                      [SMTPat (memP x (concatMap f l))]
 
 let rec concatmaplemma #a #b l f x =
@@ -66,7 +67,7 @@ let rec concatmaplemma #a #b l f x =
     concatmaplemma t f x
 
 let dm (a : Type) (wp : w a) : Type =
-  p:(a -> Type0) -> squash (wp p) -> l:(m a){forall x. memP x l ==> p x}
+  p:(a -> Type0) -> squash (wp p) -> l:(m a){forall x. {:nopattern (* override *)} memP x l ==> p x}
 
 let irepr (a : Type) (wp: w a) = dm a wp
 
@@ -76,13 +77,13 @@ let rec pmap #a #b #pre (#post:b->Type0)
   (f : (x:a -> Pure b (requires (pre x)) (ensures post)))
   (l : list a)
   : Pure (list (v:b{post v}))
-         (requires (forall x. memP x l ==> pre x))
+         (requires (forall x. {:nopattern (* override *)} memP x l ==> pre x))
          (ensures (fun _ -> True))
   = match l with
     | [] -> []
     | x::xs -> f x :: pmap #_ #_ #pre #post f xs
 
-let rec unref #a #p (l : list (v:a{p v})) : l:(list a){forall x. memP x l ==> p x} =
+let rec unref #a #p (l : list (v:a{p v})) : l:(list a){forall x. {:nopattern (* override *)} memP x l ==> p x} =
   match l with
   | [] -> []
   | x :: xs -> x :: unref xs
@@ -105,7 +106,7 @@ let rec append_memP #t l1 l2 a = match l1 with
   | hd::tl -> append_memP tl l2 a
 
 let rec flatten_mem_lem #a (l : list (list a)) (x:a)
-  : Lemma (memP x (flatten l) <==> (exists l0. memP l0 l /\ memP x l0))
+  : Lemma (memP x (flatten l) <==> (exists l0. {:nopattern (* override *)} memP l0 l /\ memP x l0))
           [SMTPat (memP x (flatten l))]
   = match l with
     | [] -> ()
@@ -113,7 +114,7 @@ let rec flatten_mem_lem #a (l : list (list a)) (x:a)
 
 let ibind (a : Type) (b : Type) (wp_v : w a) (wp_f: a -> w b) (v : irepr a wp_v) (f : (x:a -> irepr b (wp_f x))) : irepr b (w_bind wp_v wp_f) =
   fun p _ -> let l1 = v (fun x -> wp_f x p) () in
-          let l2 = pmap #_ #(list b) #(fun x -> wp_f x p) #(fun l -> forall x. memP x l ==> p x) (fun x -> f x p ()) l1 in
+          let l2 = pmap #_ #(list b) #(fun x -> wp_f x p) #(fun l -> forall x. {:nopattern (* override *)} memP x l ==> p x) (fun x -> f x p ()) l1 in
           let l2 = unref l2 in
           let l2f = List.Tot.flatten l2 in
           l2f
@@ -121,7 +122,8 @@ let ibind (a : Type) (b : Type) (wp_v : w a) (wp_f: a -> w b) (v : irepr a wp_v)
 let isubcomp (a:Type) (wp1 wp2: w a) (f : irepr a wp1) : Pure (irepr a wp2) (requires w_ord wp2 wp1) (ensures fun _ -> True) = f
 
 let wp_if_then_else (#a:Type u#a) (wp1 wp2:w a) (b:bool) : w a=
-  elim_pure_wp_monotonicity_forall u#a ();
+  elim_pure_wp_monotonicity wp1;
+  elim_pure_wp_monotonicity wp2;
   as_pure_wp (fun p -> (b ==> wp1 p) /\ ((~b) ==> wp2 p))
 
 let i_if_then_else (a : Type) (wp1 wp2 : w a) (f : irepr a wp1) (g : irepr a wp2) (b : bool) : Type =
@@ -154,7 +156,7 @@ let wrap (f:int -> ND unit (as_pure_wp (fun p -> True))) (x':int) : ND unit (as_
   | None -> f 4
 
 
-assume val f : int -> ND unit (as_pure_wp (fun p -> forall x. p x))
+assume val f : int -> ND unit (as_pure_wp (fun p -> forall x. {:nopattern (* override *)} p x))
 
 let rewrite_inside_reify (x y:int) (_:squash (x == y)) =
   assert (reify (f x) (fun _ -> True) == reify (f y) (fun _ -> True))
