tests/micro-benchmarks/Effects.Coherence.fst
@@ -38,7 +38,7 @@ new_effect M3 = M1
 
 let lift_pure_m (a:Type u#a) (wp:_) (f:unit -> PURE a wp)
   : Pure (repr a ()) (requires wp (fun _ -> True)) (ensures fun _ -> True)
-  = FStar.Monotonic.Pure.elim_pure_wp_monotonicity_forall u#a ();
+  = FStar.Monotonic.Pure.elim_pure_wp_monotonicity wp;
     f ()
 sub_effect PURE ~> M1 = lift_pure_m
 
